\documentclass[10pt,a4paper, margin=1in]{article}
\usepackage{fullpage}
\usepackage{amsfonts, amsmath, pifont}
\usepackage{amsthm}
\usepackage{graphicx}

% \usepackage[utf8]{inputenc}
\usepackage{float}
\usepackage{tkz-euclide}
\usepackage{tikz}

\usepackage{geometry}
 \geometry{
 a4paper,
 total={210mm,297mm},
 left=10mm,
 right=10mm,
 top=10mm,
 bottom=10mm,
 }
 % Write both of your names here. Fill exxxxxxx with your ceng mail address.
 \author{
  Uçan, Yiğitcan\\
  \texttt{e2310555@ceng.metu.edu.tr}
  \and
  Akın, Ozan\\
  \texttt{e2309599@ceng.metu.edu.tr}
}
\title{CENG 384 - Signals and Systems for Computer Engineers \\
Spring 2021 \\
Homework 4}
\begin{document}
\maketitle



\noindent\rule{19cm}{1.2pt}

\begin{enumerate}

\item %write the solution of q1
    \begin{enumerate}
    % Write your solutions in the following items.
    \item %write the solution of q1a
    \[ 4x(t) - 5y(t) + \int (x(t) - 6y(t)) \,dt = \frac{dy(t)}{dt} \]
    \[ 4x'(t) - 5y'(t) + x(t) - 6y(t) = y''(t) \]

    \item 
    
    \[ 4x'(t) - 5y'(t) + x(t) - 6y(t) = y''(t) \]
    \[ 4x'(t) + x(t) = y''(t) + 5y'(t) + 6y(t) \]
    \[ H(j\omega) = \frac{4j\omega + 1}{(j\omega)^2 + 5j\omega + 6} \]
    
    \item %write the solution of q1c
    
    \[ H(j\omega) = \frac{4j\omega + 1}{(j\omega)^2 + 5j\omega + 6} \]
    \[ H(j\omega) = \frac{-7}{j\omega + 2} + \frac{11}{j\omega + 3} \]
    \[ h(t) = -7 e^{-2t}u(t) + 11 e^{-3t}u(t) \]
    
    \item %write the solution of q1d
    
    \[ Y(j\omega) = X(j\omega) H(j\omega) \]
    \[ Y(j\omega) = X(j\omega) (\frac{-7}{j\omega + 2} + \frac{11}{j\omega + 3}) \]
    
    \begin{center}
        if we take $x(t) = \frac{1}{4}e^{-t/4}u(t)$ then $X(jw) = \frac{\frac{1}{4}}{j\omega + \frac{1}{4}}$
    \end{center}
    
    \[ Y(j\omega) = \frac{\frac{1}{4}}{j\omega + \frac{1}{4}} (\frac{-7}{j\omega + 2} + \frac{11}{j\omega + 3}) \]
    
    \[Y(j\omega) = \frac{1}{jw + 2} - \frac{1}{jw + 3}\]
    
    \[y(t) = e^{-2t}u(t) - e^{-3t}u(t) \]

    \end{enumerate}

\item %write the solution of q2
    \begin{enumerate}
    % Write your solutions in the following items.
    \item %write the solution of q2a
    \[H(j\omega) = \frac{j\omega + 4}{-\omega^2 + 5 j \omega + 6} = \frac{j\omega + 4}{(j\omega)^2 + 5 j \omega + 6}= \frac{j\omega + 4}{(j\omega + 3) \cdot (j\omega + 2)} \]
    
    \[ \frac{d^2y(t)}{dt^2} + 5 \frac{dy(t)}{dt} + 6y(t) = \frac{dx(t)}{dt} + 4 x(t)\]
    \item %write the solution of q2b // ex4.25
    \[H(j\omega) = \frac{j\omega + 4}{(j\omega + 3) \cdot (j\omega + 2)} = \frac{2}{j\omega+2} - \frac{1}{j\omega+3}\]
    \[h(t) = 2 e^{-2t} u(t) - e^{-3t} u(t) \]
    \item %write the solution of q2c
    \[x(t) = e^{-4t} u(t) - te^{-4t} u(t)\]
    \[ Y(j\omega) = H(j\omega)X(j\omega) = (\frac{j\omega + 4}{(j\omega + 3) \cdot (j\omega + 2)})(\frac{1}{j\omega + 4} - \frac{1}{(j\omega + 4)^2})\]
    \[ Y(j\omega) = \frac{1}{2 (j\omega + 2)} - \frac{1}{2 (j\omega + 4)}\]
    
    \item %write the solution of q2d
    \[ y(t) = (\frac{1}{2} e^{-2t} + \frac{1}{2} e^{-4t}) u(t)\]
    \end{enumerate}

\item %write the solution of q3  
    \begin{enumerate}
    % Write your solutions in the following items.
    \item %write the solution of q3a
    ~ \\
    \begin{center}
        using the property e from the week 10 notes table 2.
    \end{center}
    
    \[ X(j\omega) = \frac{2}{\omega^2 + 1}\]
    
    \item %write the solution of q3b
    
    \[ X(j\omega) = j \frac{d}{d\omega} X(j\omega) \]
    \[ X(j\omega) = j \cdot \frac{-4\omega}{(\omega^2 + 1)^2} \]
    \[ X(j\omega) = \frac{-4\omega j}{(\omega^2 + 1)^2} \]
    
    \item %write the solution of q3c
    
    \[ X(j\omega) = \frac{-4\omega j}{(\omega^2 + 1)^2} \]
    \[ X(j\omega) = \frac{-4\omega j}{(-(j\omega)^2 + 1)^2} \]
    
    \end{enumerate}

\item %write the solution of q4
    \begin{enumerate}
    % Write your solutions in the following items.
    \item %write the solution of q4a
    \[ y[n] = -\frac{y[n-2]}{8} + \frac{3y[n-1]}{4} + 2x[n]\]
    \[ y[n] - \frac{3y[n-1]}{4} + \frac{y[n-2]}{8} = 2x[n]\]
    \item %write the solution of q4b          c                 
    \[H(e^{j\omega}) = \frac{2}{1 - \frac{3}{4} e^{-j\omega}+ \frac{1}{8} e^{-2j\omega} }\]
    \item %write the solution of q4c
    \[H(e^{j\omega}) = \frac{16}{(e^{-j\omega} -2) (e^{-j\omega} -4) }\]
    
    Partial fraction expansion:
    
    \[H(e^{j\omega}) = \frac{8}{e^{-j\omega} - 4} - \frac{8}{e^{-j\omega} - 2}\]
    
    \[H(e^{j\omega}) = \frac{-2}{1 - \frac{1}{4} e^{-j\omega}} + \frac{4}{1 - \frac{1}{2}e^{-j\omega}}\]
    
    \[h[n] = 4(\frac{1}{2})^n \cdot u[n] -2(\frac{1}{4})^n \cdot u[n]\]
    
    \item %write the solution of q4d
    
    \[ x[n] = (\frac{1}{4})^n u[n]\]
    
    \[ Y(e^{j\omega}) = H(e^{j\omega})X(e^{j\omega}) = (\frac{-2}{1 - \frac{1}{4} e^{-j\omega}} + \frac{4}{1 - \frac{1}{2}e^{-j\omega}}) (\frac{1}{1-\frac{1}{4}e^{-j\omega}})\]
    
    
    \[ Y(e^{j\omega}) = \frac{4}{1-\frac{1}{4}e^{-j\omega}} -  \frac{2}{(1-\frac{1}{4}e^{-j\omega})^2}+ \frac{8}{1-\frac{1}{2}e^{-j\omega}}\]
    
    \[y[n] = (-4(\frac{1}{4})^n- 2(n+1)(\frac{1}{4})^n + 8 (\frac{1}{2})^n) u[n] \]
    
    \end{enumerate}

\item %write the solution of q5
    \[H(e^{j\omega}) = \frac{5e^{-j\omega} - 12}{e^{-2j\omega} - 7 e^{-j\omega} + 12}\]
    \[H(e^{j\omega}) = \frac{5e^{-j\omega} - 12}{(e^{-j\omega} - 3)(e^{-j\omega} - 4)}\]
    \[H(e^{j\omega}) = \frac{8}{e^{-j\omega} - 4} - \frac{3}{e^{-j\omega} - 3}\]
    \[H(e^{j\omega}) = \frac{1}{1 - \frac{1}{3} e^{-j\omega}} - \frac{2}{1 - \frac{1}{4} e^{-j\omega}}\]
    
    \[ h[n] = h_1[n] + h_2[n] = (\frac{1}{3})^n \cdot u[n] - 2 (\frac{1}{4})^n \cdot u[n] \]
    
    \[ h_1[n] = (\frac{1}{3})^n \cdot u[n] \]
    \[ h_2[n] = -2 (\frac{1}{4})^n \cdot u[n] \]
    

\item %write the solution of q6
    \begin{enumerate}
    % Write your solutions in the following items.
    \item %write the solution of q6a ex5.19
    \[H(e^{j\omega}) = \frac{1}{1-\frac{e^{-j\omega}}{6} - \frac{e^{-2j\omega}}{6} } \]
    
    \[ H(e^{j\omega}) = \frac{Y(e^{j\omega})}{X(e^{j\omega})}\]
    
    \[ y[n] - \frac{1}{6}y[n-1] - \frac{1}{6}y[n-2] = x[n]\]
    \item %write the solution of q6b
    
    \[ y[n] = \frac{1}{6}y[n-1] + \frac{1}{6}y[n-2] + x[n]\]
    
\begin{center}
	\tikzset{%
		block/.style    = {draw, thick, rectangle, minimum height = 3em,
			minimum width = 3em},
		sum/.style      = {draw, circle, node distance = 2cm}, % Adder
		input/.style    = {coordinate}, % Input
		output/.style   = {coordinate} % Output
	}
	% Defining string as labels of certain blocks.
	\newcommand{\suma}{\Large$+$}
	\newcommand{\inte}{$\displaystyle \int$}
	\newcommand{\derv}{\huge$\frac{d}{dt}$}
	
	\begin{tikzpicture}[auto, thick, node distance=2cm, >=triangle 45]
	\draw
	% Drawing the blocks of first filter :
	node at (0, 0) [input] (inp) {\Large \textopenbullet}
	node [sum, right of=inp] (sum) {\suma}
	node [output, right of=sum] (out) {}
	node [block, below of=out] (dec) {$D$}
	node [block, below of=dec] (dec2) {$D$}
	node [output, right of=out] (out2) {\Large \textopenbullet}
	node [sum, below of=sum] (temp) {\suma}
	node [output, below of=temp] (temp2) {}
	;
	\draw[->](inp) -- node{$x[n]$} (sum);
	\draw[-](sum) -- (out);
	\draw[->](out) -- node{$y[n]$} (out2);
	\draw[->](out) -- (dec);
	\draw[->](dec) -- (dec2);
	\draw[->](dec) -- node{$\frac{1}{6}$} (temp);
	\draw[-](dec2) -- node{$\frac{1}{6}$} (temp2);
	\draw[->](temp2) -- (temp);
	\draw[->](temp) -- (sum);
	\end{tikzpicture}
\end{center}

    \item %write the solution of q6c ex5.19
    
    \[H(e^{j\omega}) = \frac{1}{1-\frac{e^{-j\omega}}{6} - \frac{e^{-2j\omega}}{6} } =  \frac{6}{6-e^{-j\omega} - e^{-2j\omega} }\]
    
    \[H(e^{j\omega}) = \frac{6}{(3+e^{-j\omega})(2-e^{-j\omega})}\]
    
    Partial fraction expansion:
    
    \[H(e^{j\omega}) = \frac{2}{5} \cdot \frac{1}{1 + \frac{1}{3} e^{-j\omega}} + \frac{3}{5} \cdot \frac{1}{1 - \frac{1}{2} e^{-j\omega}} \]
    
    \[h[n] = \frac{2}{5} \cdot (-\frac{1}{3})^n \cdot u[n] + \frac{3}{5} \cdot (\frac{1}{2})^n \cdot u[n]\]
    \end{enumerate}    

\end{enumerate}
\end{document}

